Fix extraction process

io/TC.MLify.IIOwp.fst
@@ -14,56 +14,23 @@ open Free
 open IO.Sig
 open DM.IIO
 
-(** To be able to mlify IIOwp, the weakest-precondition of the computation must be
-    (fun p h -> True) -- this is the weakest weakest-precondition.
-
-    Previous code required (fun p h -> forall lt r. p lt r). I tought that this guarantees 
-     `p lt r` without any requirements, but it actually requires that p should be valid for 
-     all lts and rs. 
-**)
-
 exception Something_went_really_bad
 
-let lemma_continuation_is_weak (tree:dm_iio 'a (weakest_hist ())) (pre:pure_pre) (proof:squash pre) (k:(squash pre -> iio 'a)) :
-  Lemma
-    (requires (PartialCall? tree /\ PartialCall?.pre tree == pre /\ PartialCall?.cont tree == k))
-    (ensures (weakest_hist () `hist_ord` (dm_iio_theta (k proof)))) =
-  calc (hist_ord #event #'a) {
-    weakest_hist ();
-    `hist_ord` {}
-    dm_iio_theta tree;
-    `hist_ord` {}
-    dm_iio_theta (PartialCall pre k);
-    `hist_ord` {}
-    hist_bind (DMFree.partial_call_wp pre) (fun r -> dm_iio_theta (k r));
-    `hist_ord` {}
-    dm_iio_theta (k proof);
-  }
+(** the_p is used at the spec level and they are used to instantiate later the 
+    refinement of the DM: wp `hist_ord` theta m. By instantiating the refinement, we get:
+    forall h. True ==> theta m (the_p ()) h, thus getting theta m. 
+    It is important that the_p is defined as such to get True as pre-condition. **)
+let the_p #a () : hist_post #event a = fun _ _ -> True
 
-let rec skip_partial_calls (tree:dm_iio 'a (weakest_hist ())) : ML 'a =
+let rec skip_partial_calls (tree:iio 'a) (_:squash (forall h. dm_iio_theta tree (the_p ()) h)) : ML 'a =
   match tree with
   | Return y -> y
   | PartialCall pre k -> begin
     (** The intuition here is that the pre-condition is true,
     thus, all asserts are true **)
-    (** the following assert is the refinement hidden by the dm **)
-    assert (forall p h. weakest_hist #'a #event () p h ==> dm_iio_theta tree p h);
-    assert (forall p h. dm_iio_theta tree p h);
-    assert (forall p h. dm_iio_theta tree p h ==> pre);
-    assert (forall (p:hist_post #event 'a) (h:trace). pre) by (
-      let p = FStar.Tactics.forall_intro () in
-      let h = FStar.Tactics.forall_intro () in
-      mapply (ExtraTactics.instantiate_multiple_foralls (nth_binder (-7)) [binder_to_term p;binder_to_term h]);
-      ignore (ExtraTactics.instantiate_multiple_foralls (nth_binder (-14)) [binder_to_term p;binder_to_term h]);
-      assumption ());
-    assert (pre) by (
-      ignore (ExtraTactics.instantiate_multiple_foralls (nth_binder (-1)) [(`(fun _ _ -> True)); (`[])]);
-      assumption ()
-    );
-    let proof : squash pre = () in
-    lemma_continuation_is_weak tree pre proof k;
-    let tree' : dm_iio 'a (weakest_hist ()) = k proof in
-   skip_partial_calls tree'
+   assert (dm_iio_theta tree (the_p ()) []);
+   assert pre;
+   skip_partial_calls (k ()) ()
   end
   (** during extraction, Free.IO.Call is replaced with an actual
   implementation of the commands, therefore, the `Call` constructor
@@ -73,13 +40,13 @@ let rec skip_partial_calls (tree:dm_iio 'a (weakest_hist ())) : ML 'a =
 
 instance mlifyable_iiowp
   t1 t2 {| ml t1 |} {| ml t2 |} :
-  Tot (mlifyable (t1 -> IIOwp t2 (weakest_hist ()))) =
+  Tot (mlifyable (t1 -> IIOwp t2 (trivial_hist ()))) =
   mk_mlifyable
-    #(t1 -> IIOwp t2 (weakest_hist ()))
+    #(t1 -> IIOwp t2 (trivial_hist ()))
     (t1 -> ML t2)
     (fun f x -> 
-     let tree : dm_iio t2 (weakest_hist ()) = reify (f x) in
-     skip_partial_calls tree)
+     let tree : dm_iio t2 (trivial_hist ()) = reify (f x) in
+     skip_partial_calls tree ())
 
 (** Ideas to improve mlifyable_iio_miio:
 1. What if instead of Tot, we use Ex, to be able to internalize try_catch.
@@ -97,11 +64,11 @@ instance mlifyable_iiowp
 instance mlifyable_inst_iiowp
   t1 t3
   {| d1:instrumentable t1 |} {| d2:ml t3 |} :
-  Tot (mlifyable (t1 -> IIOwp t3 (weakest_hist ()))) =
+  Tot (mlifyable (t1 -> IIOwp t3 (trivial_hist ()))) =
   mk_mlifyable
     #_
     (d1.start_type -> ML t3)
     #(ml_ml_arrow_1 d1.start_type t3 #d1.start_type_c #d2)
-    (fun (p:t1 -> IIOwp t3 (weakest_hist ())) (ct:d1.start_type) ->
-     let tree : dm_iio t3 (weakest_hist ()) = reify (p (d1.instrument ct)) in
-     skip_partial_calls tree)
+    (fun (p:t1 -> IIOwp t3 (trivial_hist ())) (ct:d1.start_type) ->
+     let tree : dm_iio t3 (trivial_hist ()) = reify (p (d1.instrument ct)) in
+     skip_partial_calls tree ())
